proofs of assumption (actually eassumption)

theories/RTac/Assumption.v
@@ -6,7 +6,6 @@ Require Import MirrorCore.ExprI.
 Require Import MirrorCore.SubstI.
 Require Import MirrorCore.ExprDAs.
 Require Import MirrorCore.RTac.Core.
-Require Import MirrorCore.RTac.RunOnGoals.
 
 Require Import MirrorCore.Util.Forwardy.
 
@@ -36,31 +35,41 @@ Section parameterized.
   End findHyp.
 
   Context {RType_typ : RType typ}.
+  Context {RTypeOk_typ : RTypeOk}.
   Context {Expr_expr : Expr RType_typ expr}.
+  Context {ExprOk_expr : ExprOk Expr_expr}.
   Context {Typ0_Prop : Typ0 _ Prop}.
 
-  Variable check : forall {subst : Type} {S : Subst subst expr},
+  Variable check : forall {subst : Type} {S : Subst subst expr} {SU : SubstUpdate subst expr},
                      Ctx typ expr -> expr -> expr -> subst -> option subst.
+  Variable mentionsAny : (nat -> bool) -> (nat -> bool) -> expr -> bool.
+  Variable instantiate : (nat -> option expr) -> nat -> expr -> expr.
 
-  Definition ASSUMPTION : rtac typ expr :=
+  Let SubstUpdate_ctx_subst ctx :=
+    @SubstUpdate_ctx_subst _ _ _ _ instantiate mentionsAny ctx.
+  Local Existing Instance SubstUpdate_ctx_subst.
+
+
+  Definition EASSUMPTION : rtac typ expr :=
     fun _ _ _ _ ctx s gl =>
-      match @findHyp (ctx_subst ctx) (fun e => @check _ _ ctx gl e s) ctx with
+      match @findHyp (ctx_subst ctx)
+                     (fun e => @check _ _ _ ctx gl e s) ctx with
         | None => Fail
         | Some s' => Solved s'
       end.
 
-(*
   Hypothesis checkOk
   : forall ctx e1 e2 s s',
-      check ctx e1 e2 s = Some s' ->
+      @check (ctx_subst ctx) _ _ ctx e1 e2 s = Some s' ->
       WellFormed_subst s ->
-      let tus := getUVars ctx nil in
-      let tvs := getVars ctx nil in
+      let tus := getUVars ctx in
+      let tvs := getVars ctx in
       WellFormed_subst s' /\
       forall v1 v2 sD,
-        exprD' tus tvs e1 (@typ0 _ _ Prop _) = Some v1 ->
-        exprD' tus tvs e1 (@typ0 _ _ Prop _) = Some v2 ->
+        propD tus tvs e1 = Some v1 ->
+        propD tus tvs e2 = Some v2 ->
         substD tus tvs s = Some sD ->
+        substR tus tvs s s' /\
         exists sD',
              substD tus tvs s' = Some sD'
           /\ forall us vs,
@@ -69,59 +78,86 @@ Section parameterized.
                v1 us vs = v2 us vs.
 
   Lemma findHypOk
-  : forall ctx tus tvs g s s',
-      findHyp (check ctx (** TODO: This isn't right **) g) ctx s = Some s' ->
+  : forall g (ctx ctx' : Ctx typ expr)
+           (s s' : ctx_subst (Ctx_append ctx ctx')),
+      findHyp (T:=ctx_subst (Ctx_append ctx ctx'))
+              (fun g' => @check _ _ _ (Ctx_append ctx ctx') g g' s)
+              ctx = Some s' ->
+      getAmbient ctx' = getEnvs ctx ->
       WellFormed_subst s ->
       WellFormed_subst s' /\
-      let tus' := tus ++ getUVars ctx nil in
-      let tvs' := tvs ++ getVars ctx nil in
-      match propD  tus' tvs' g
-          , substD tus' tvs' s
-          , substD tus' tvs' s'
+      match propD  _ _ g
+          , pctxD s
+          , pctxD s'
       with
         | Some gD , Some sD , Some sD' =>
-          ctxD' ctx (fun (us : hlist _ (rev tus')) (vs : hlist _ (rev tvs')) =>
-                       let us := hlist_unrev us in
-                       let vs := hlist_unrev vs in
-                       sD' us vs ->
-                       sD us vs /\ gD us vs)
+          SubstMorphism s s' /\
+          forall us vs, sD' gD us vs
         | None , _ , _
         | _ , None , _ => True
         | Some _ , Some _ , None => False
       end.
-(*
   Proof.
     induction ctx; simpl; intros; try congruence.
-    { specialize (IHctx tus (tvs ++ t :: nil) _ _ _ H H0).
-      forward_reason; split; eauto.
-      forward.
-      subst.
-      eapply substD_weakenV with (tvs' := t :: nil) in H4.
-      eapply exprD'_typ0_weakenV with (tvs' := t :: nil) in H3.
-      forward_reason.
-      rewrite H4 in H2.
-      change_rewrite H3 in H2.
-      forwardy.
-      rewrite
- }
-    { specialize (IHctx (tus ++ t :: nil) tvs _ _ _ H H0).
-      forward_reason; split; eauto.
-      forward.
-      subst. eapply H4. }
-    { consider (check ctx g e s); intros.
-      { clear IHctx. inv_all; subst.
+    { specialize (@IHctx (Ctx_append (CAll (CTop (getUVars ctx) (getVars ctx)) t) ctx')).
+      rewrite Ctx_append_assoc in IHctx. simpl in IHctx.
+      destruct (IHctx s s' H); eauto.
+      simpl in *.
+      rewrite getAmbient_Ctx_append. simpl.
+      symmetry. apply getEnvs_getUVars_getVars. }
+    { specialize (@IHctx (Ctx_append (CExs (CTop (getUVars ctx) (getVars ctx)) t) ctx')).
+      rewrite Ctx_append_assoc in IHctx. simpl in IHctx.
+      destruct (IHctx s s' H); eauto.
+      simpl in *.
+      rewrite getAmbient_Ctx_append. simpl.
+      symmetry. apply getEnvs_getUVars_getVars. }
+    { consider (check (Subst_ctx_subst (Ctx_append (CHyp ctx e) ctx'))
+          (SubstUpdate_ctx_subst (Ctx_append (CHyp ctx e) ctx'))
+          (Ctx_append (CHyp ctx e) ctx') g e s); intros.
+      { inv_all; subst.
+        clear IHctx.
         eapply checkOk in H; clear checkOk; eauto.
-        forward_reason; split; eauto.
+        forward_reason; split; auto.
         forward.
-        destruct o0; inv_all; subst.
-*)
-  Admitted.
-*)
+        destruct (pctxD_substD H1 H4) as [ ? [ ? ? ] ].
+        specialize (fun v2 H => @H3 _ v2 _ eq_refl H H5).
+        destruct (pctxD_get_hyp _ _ _ H1 H4) as [ ? [ ? ? ] ].
+        change (getUVars ctx) with (getUVars (CHyp ctx e)) in H7.
+        change (getVars ctx) with (getVars (CHyp ctx e)) in H7.
+        eapply propD_weaken_by_Ctx_append in H7; eauto.
+        forward_reason.
+        eapply H3 in H7.
+        forward_reason.
+        destruct (substD_pctxD _ H H4 H10) as [ ? [ ? ? ] ].
+        rewrite H12. split; try eassumption.
+        intros. gather_facts.
+        eapply pctxD_SubstMorphism; [ eapply H7 | |  | ]; eauto.
+        gather_facts.
+        eapply Pure_pctxD; eauto.
+        clear - H11 H9.
+        intros; eauto.
+        eapply H11 in H1.
+        destruct H1. rewrite H2; clear H2.
+        eapply H9. eauto. }
+      { specialize (@IHctx (Ctx_append (CHyp (CTop (getUVars ctx) (getVars ctx)) e) ctx')).
+        rewrite Ctx_append_assoc in IHctx. simpl in *.
+        eapply IHctx; eauto.
+        rewrite getAmbient_Ctx_append. simpl.
+        symmetry. eapply getEnvs_getUVars_getVars. } }
+  Qed.
 
-  Theorem ASSUMPTION_sound : rtac_sound ASSUMPTION.
+  Theorem ASSUMPTION_sound : rtac_sound EASSUMPTION.
   Proof.
-    unfold ASSUMPTION, rtac_sound.
+    unfold EASSUMPTION, rtac_sound.
     intros. subst.
-  Admitted.
+    red. simpl.
+    forward.
+    eapply findHypOk with (ctx' := CTop (getUVars ctx) (getVars ctx)) in H; eauto.
+    { forward_reason; split; auto.
+      forward. clear - H2 H3. exfalso.
+      change_rewrite H2 in H3. congruence. }
+    { simpl. symmetry.
+      eapply getEnvs_getUVars_getVars. }
+  Qed.
 
 End parameterized.
